src/proof/controllers/statefulset/outdated.v
@@ -58,7 +58,7 @@ Proof.
   - rewrite /PodSpecV.deepown /without_statefulset_fields /=.
     iSplit; first done.
     iSplitL.
-    + iExists []. rewrite /deepown_list big_sepL2_nil.
+    + iExists []. rewrite /deepown_list_dq big_sepL2_nil.
       iSplit; [iApply own_slice_nil|done].
     + done.
 Qed.
