src/proof/kubernetes_types/persist.v
@@ -1,0 +1,239 @@
+(* Discarding fractions of deep ownership.
+
+   The concurrent pod-creating goroutines of the ReplicaSet controller read the
+   ReplicaSet's ObjectMeta and pod template simultaneously. Sharing those reads
+   across goroutines requires the corresponding deep-ownership predicates to be
+   persistent, which we obtain by discarding the fraction ([DfracDiscarded]).
+   This file proves the discard lemmas and persistence instances for the
+   predicates involved. *)
+From New.proof Require Import prelude empty_ffi.
+From New.proof.kubernetes_types Require Export pod replicaset.
+From New.proof Require Import proof_prelude.
+
+Section persist.
+Context `{hG: !heapGS Σ} `{!ffi_semantics _ _}.
+Context {sem : go.Semantics}
+  {meta_v1_sem : code.k8s_io.apimachinery.pkg.apis.meta.v1.v1.Assumptions}
+  {core_v1_sem : code.k8s_io.api.core.v1.v1.Assumptions}
+  {apps_v1_sem : code.k8s_io.api.apps.v1.v1.Assumptions}.
+
+(* [TimeV.deepown] and [ManagedFieldsEntryV.deepown] are opaque in the pure
+   model (see kubernetes_types/common.v and objectmeta.v). We assume they are
+   ownership predicates in the usual sense: any fraction can be discarded to
+   obtain persistent, read-only knowledge. Every points-to based instantiation
+   of these predicates satisfies both assumptions. *)
+Axiom time_deepown_persist : ∀ c v dq,
+  (TimeV.deepown c v dq : iProp Σ) ⊢ |==> TimeV.deepown c v DfracDiscarded.
+Axiom time_deepown_persistent : ∀ c v,
+  Persistent (TimeV.deepown c v DfracDiscarded : iProp Σ).
+#[global] Existing Instance time_deepown_persistent.
+Axiom managed_fields_entry_deepown_persist : ∀ c v dq,
+  (ManagedFieldsEntryV.deepown c v dq : iProp Σ) ⊢ |==> ManagedFieldsEntryV.deepown c v DfracDiscarded.
+Axiom managed_fields_entry_deepown_persistent : ∀ c v,
+  Persistent (ManagedFieldsEntryV.deepown c v DfracDiscarded : iProp Σ).
+#[global] Existing Instance managed_fields_entry_deepown_persistent.
+
+Lemma big_sepL2_persist {A B} (P : A → B → dfrac → iProp Σ) dq (cs : list A) (vs : list B) :
+  (∀ c v, P c v dq ⊢ |==> P c v DfracDiscarded) →
+  ([∗ list] c;v ∈ cs;vs, P c v dq) ⊢ |==> [∗ list] c;v ∈ cs;vs, P c v DfracDiscarded.
+Proof.
+  intros HP.
+  iInduction cs as [|c cs] "IH" forall (vs); destruct vs as [|v vs].
+  - rewrite !big_sepL2_nil. iIntros "_". iModIntro. done.
+  - iIntros "H". iDestruct (big_sepL2_nil_inv_l with "H") as %Hnil. discriminate Hnil.
+  - iIntros "H". iDestruct (big_sepL2_nil_inv_r with "H") as %Hnil. discriminate Hnil.
+  - rewrite !big_sepL2_cons. iIntros "[Hc Hcs]".
+    iMod (HP with "Hc") as "Hc". iMod ("IH" with "Hcs") as "Hcs".
+    iModIntro. by iFrame.
+Qed.
+
+Lemma owner_reference_deepown_persist c v dq :
+  OwnerReferenceV.deepown c v dq ⊢ |==> OwnerReferenceV.deepown c v DfracDiscarded.
+Proof.
+  rewrite /OwnerReferenceV.deepown. iNamed 1.
+  iAssert (|==> match v.(OwnerReferenceV.Controller') with
+    | Some vc => ∃ cc, c.(v1.OwnerReference.Controller') ↦□ cc ∗ ⌜ cc = vc ⌝
+    | None => True%I
+    end)%I with "[Hdeepown_controller_some]" as ">Hcontroller".
+  { destruct (v.(OwnerReferenceV.Controller')) as [vc|]; last done.
+    iDestruct "Hdeepown_controller_some" as (cc) "[Hcc %Hcc]".
+    iPersist "Hcc". iModIntro. iExists cc. by iFrame "# %". }
+  iAssert (|==> match v.(OwnerReferenceV.BlockOwnerDeletion') with
+    | Some vb => ∃ cb, c.(v1.OwnerReference.BlockOwnerDeletion') ↦□ cb ∗ ⌜ cb = vb ⌝
+    | None => True%I
+    end)%I with "[Hdeepown_blockownerdeleton_some]" as ">Hblock".
+  { destruct (v.(OwnerReferenceV.BlockOwnerDeletion')) as [vb|]; last done.
+    iDestruct "Hdeepown_blockownerdeleton_some" as (cb) "[Hcb %Hcb]".
+    iPersist "Hcb". iModIntro. iExists cb. by iFrame "# %". }
+  iModIntro. by iFrame "∗ # %".
+Qed.
+
+#[global] Instance owner_reference_deepown_persistent c v :
+  Persistent (OwnerReferenceV.deepown c v DfracDiscarded).
+Proof.
+  rewrite /OwnerReferenceV.deepown.
+  destruct (v.(OwnerReferenceV.Controller')), (v.(OwnerReferenceV.BlockOwnerDeletion'));
+    apply _.
+Qed.
+
+Lemma objectmeta_deepown_persist c v dq :
+  ObjectMetaV.deepown c v dq ⊢ |==> ObjectMetaV.deepown c v DfracDiscarded.
+Proof.
+  rewrite /ObjectMetaV.deepown. iNamed 1.
+  iMod (time_deepown_persist with "Hdeepown_creationtimestamp") as "Hdeepown_creationtimestamp".
+  iAssert (|==> match v.(ObjectMetaV.DeletionTimestamp') with
+    | Some vd => ∃ cd, c.(v1.ObjectMeta.DeletionTimestamp') ↦□ cd ∗ TimeV.deepown cd vd DfracDiscarded
+    | None => True%I
+    end)%I with "[Hdeepown_deletiontimestamp_some]" as ">Hdeletiontimestamp".
+  { destruct (v.(ObjectMetaV.DeletionTimestamp')) as [vd|]; last done.
+    iDestruct "Hdeepown_deletiontimestamp_some" as (cd) "[Hcd Ht]".
+    iPersist "Hcd". iMod (time_deepown_persist with "Ht") as "Ht".
+    iModIntro. iExists cd. by iFrame "∗ #". }
+  iAssert (|==> match v.(ObjectMetaV.DeletionGracePeriodSeconds') with
+    | Some vd => ∃ cd, c.(v1.ObjectMeta.DeletionGracePeriodSeconds') ↦□ cd ∗ ⌜ cd = vd ⌝
+    | None => True%I
+    end)%I with "[Hdeepown_deletiongraceperiodseconds_some]" as ">Hgrace".
+  { destruct (v.(ObjectMetaV.DeletionGracePeriodSeconds')) as [vd|]; last done.
+    iDestruct "Hdeepown_deletiongraceperiodseconds_some" as (cd) "[Hcd %Hcd]".
+    iPersist "Hcd". iModIntro. iExists cd. by iFrame "# %". }
+  iAssert (|==> match v.(ObjectMetaV.Labels') with
+    | Some vl => ∃ cl, c.(v1.ObjectMeta.Labels') ↦${DfracDiscarded} cl ∗ ⌜ cl = vl ⌝
+    | None => True%I
+    end)%I with "[Hdeepown_labels_some]" as ">Hlabels".
+  { destruct (v.(ObjectMetaV.Labels')) as [vl|]; last done.
+    iDestruct "Hdeepown_labels_some" as (cl) "[Hcl %Hcl]".
+    iMod (own_map_persist with "Hcl") as "Hcl". iModIntro. iExists cl. by iFrame "∗ %". }
+  iAssert (|==> match v.(ObjectMetaV.Annotations') with
+    | Some va => ∃ ca, c.(v1.ObjectMeta.Annotations') ↦${DfracDiscarded} ca ∗ ⌜ ca = va ⌝
+    | None => True%I
+    end)%I with "[Hdeepown_annotations_some]" as ">Hannotations".
+  { destruct (v.(ObjectMetaV.Annotations')) as [va|]; last done.
+    iDestruct "Hdeepown_annotations_some" as (ca) "[Hca %Hca]".
+    iMod (own_map_persist with "Hca") as "Hca". iModIntro. iExists ca. by iFrame "∗ %". }
+  iAssert (|==> match v.(ObjectMetaV.OwnerReferences') with
+    | Some vos => ∃ cos, c.(v1.ObjectMeta.OwnerReferences') ↦*{DfracDiscarded} cos ∗
+        [∗ list] co;vo ∈ cos;vos, OwnerReferenceV.deepown co vo DfracDiscarded
+    | None => True%I
+    end)%I with "[Hdeepown_ownerreferences_some]" as ">Howners".
+  { destruct (v.(ObjectMetaV.OwnerReferences')) as [vos|]; last done.
+    iDestruct "Hdeepown_ownerreferences_some" as (cos) "[Hcos Hlist]".
+    iMod (own_slice_persist with "Hcos") as "Hcos".
+    iMod (big_sepL2_persist OwnerReferenceV.deepown with "Hlist") as "Hlist".
+    { intros. apply owner_reference_deepown_persist. }
+    iModIntro. iExists cos. by iFrame. }
+  iAssert (|==> match v.(ObjectMetaV.Finalizers') with
+    | Some vfs => ∃ cfs, c.(v1.ObjectMeta.Finalizers') ↦*{DfracDiscarded} cfs ∗ ⌜ cfs = vfs ⌝
+    | None => True%I
+    end)%I with "[Hdeepown_finalizers_some]" as ">Hfinalizers".
+  { destruct (v.(ObjectMetaV.Finalizers')) as [vfs|]; last done.
+    iDestruct "Hdeepown_finalizers_some" as (cfs) "[Hcfs %Hcfs]".
+    iMod (own_slice_persist with "Hcfs") as "Hcfs". iModIntro. iExists cfs. by iFrame "∗ %". }
+  iAssert (|==> match v.(ObjectMetaV.ManagedFields') with
+    | Some vms => ∃ cms, c.(v1.ObjectMeta.ManagedFields') ↦*{DfracDiscarded} cms ∗
+        [∗ list] cm;vm ∈ cms;vms, ManagedFieldsEntryV.deepown cm vm DfracDiscarded
+    | None => True%I
+    end)%I with "[Hdeepown_managedfields_some]" as ">Hmanaged".
+  { destruct (v.(ObjectMetaV.ManagedFields')) as [vms|]; last done.
+    iDestruct "Hdeepown_managedfields_some" as (cms) "[Hcms Hlist]".
+    iMod (own_slice_persist with "Hcms") as "Hcms".
+    iMod (big_sepL2_persist ManagedFieldsEntryV.deepown with "Hlist") as "Hlist".
+    { intros. apply managed_fields_entry_deepown_persist. }
+    iModIntro. iExists cms. by iFrame. }
+  iModIntro. by iFrame "∗ # %".
+Qed.
+
+#[global] Instance objectmeta_deepown_persistent c v :
+  Persistent (ObjectMetaV.deepown c v DfracDiscarded).
+Proof.
+  rewrite /ObjectMetaV.deepown.
+  destruct (v.(ObjectMetaV.DeletionTimestamp')), (v.(ObjectMetaV.DeletionGracePeriodSeconds')),
+    (v.(ObjectMetaV.Labels')), (v.(ObjectMetaV.Annotations')), (v.(ObjectMetaV.OwnerReferences')),
+    (v.(ObjectMetaV.Finalizers')), (v.(ObjectMetaV.ManagedFields'));
+    apply _.
+Qed.
+
+Lemma objectmeta_deepown_l_persist l v dq :
+  ObjectMetaV.deepown_l l v dq ⊢ |==> ObjectMetaV.deepown_l l v DfracDiscarded.
+Proof.
+  iDestruct 1 as (c) "[Hl Hdeepown]".
+  iPersist "Hl". iMod (objectmeta_deepown_persist with "Hdeepown") as "Hdeepown".
+  iModIntro. iExists c. by iFrame "∗ #".
+Qed.
+
+#[global] Instance objectmeta_deepown_l_persistent l v :
+  Persistent (ObjectMetaV.deepown_l l v DfracDiscarded).
+Proof. rewrite /ObjectMetaV.deepown_l. apply _. Qed.
+
+Lemma volume_source_deepown_persist c v dq :
+  VolumeSourceV.deepown c v dq ⊢ |==> VolumeSourceV.deepown c v DfracDiscarded.
+Proof.
+  rewrite /VolumeSourceV.deepown. iNamed 1.
+  iAssert (|==> match v.(VolumeSourceV.PersistentVolumeClaim') with
+    | Some pvc => ∃ c_pvc, c.(v1.VolumeSource.PersistentVolumeClaim') ↦□ c_pvc ∗ ⌜ c_pvc = pvc ⌝
+    | None => True%I
+    end)%I with "[Hdeepown_persistentvolumeclaim_some]" as ">Hpvc".
+  { destruct (v.(VolumeSourceV.PersistentVolumeClaim')) as [pvc|]; last done.
+    iDestruct "Hdeepown_persistentvolumeclaim_some" as (c_pvc) "[Hc %Hc]".
+    iPersist "Hc". iModIntro. iExists c_pvc. by iFrame "# %". }
+  iModIntro. by iFrame "∗ # %".
+Qed.
+
+#[global] Instance volume_source_deepown_persistent c v :
+  Persistent (VolumeSourceV.deepown c v DfracDiscarded).
+Proof.
+  rewrite /VolumeSourceV.deepown. destruct (v.(VolumeSourceV.PersistentVolumeClaim')); apply _.
+Qed.
+
+Lemma volume_deepown_persist c v dq :
+  VolumeV.deepown c v dq ⊢ |==> VolumeV.deepown c v DfracDiscarded.
+Proof.
+  rewrite /VolumeV.deepown. iNamed 1.
+  iMod (volume_source_deepown_persist with "Hdeepown_volumesource") as "Hdeepown_volumesource".
+  iModIntro. by iFrame "∗ # %".
+Qed.
+
+#[global] Instance volume_deepown_persistent c v :
+  Persistent (VolumeV.deepown c v DfracDiscarded).
+Proof. rewrite /VolumeV.deepown. apply _. Qed.
+
+Lemma pod_spec_deepown_persist c v dq :
+  PodSpecV.deepown c v dq ⊢ |==> PodSpecV.deepown c v DfracDiscarded.
+Proof.
+  rewrite /PodSpecV.deepown. iNamed 1.
+  iDestruct "Hdeepown_volumes" as (volumes) "[Hsl Hlist]".
+  iMod (own_slice_persist with "Hsl") as "Hsl".
+  iMod (big_sepL2_persist VolumeV.deepown with "Hlist") as "Hlist".
+  { intros. apply volume_deepown_persist. }
+  iModIntro. iFrame "%". iExists volumes. rewrite /deepown_list_dq. by iFrame.
+Qed.
+
+#[global] Instance pod_spec_deepown_persistent c v :
+  Persistent (PodSpecV.deepown c v DfracDiscarded).
+Proof. rewrite /PodSpecV.deepown /deepown_list_dq. apply _. Qed.
+
+Lemma pod_template_spec_deepown_persist c v dq :
+  PodTemplateSpecV.deepown c v dq ⊢ |==> PodTemplateSpecV.deepown c v DfracDiscarded.
+Proof.
+  rewrite /PodTemplateSpecV.deepown. iNamed 1.
+  iMod (objectmeta_deepown_persist with "Hdeepown_objectmeta") as "Hdeepown_objectmeta".
+  iMod (pod_spec_deepown_persist with "Hdeepown_spec") as "Hdeepown_spec".
+  iModIntro. by iFrame.
+Qed.
+
+#[global] Instance pod_template_spec_deepown_persistent c v :
+  Persistent (PodTemplateSpecV.deepown c v DfracDiscarded).
+Proof. rewrite /PodTemplateSpecV.deepown. apply _. Qed.
+
+Lemma pod_template_spec_deepown_l_persist l v dq :
+  PodTemplateSpecV.deepown_l l v dq ⊢ |==> PodTemplateSpecV.deepown_l l v DfracDiscarded.
+Proof.
+  iDestruct 1 as (c) "[Hl Hdeepown]".
+  iPersist "Hl". iMod (pod_template_spec_deepown_persist with "Hdeepown") as "Hdeepown".
+  iModIntro. iExists c. by iFrame "∗ #".
+Qed.
+
+#[global] Instance pod_template_spec_deepown_l_persistent l v :
+  Persistent (PodTemplateSpecV.deepown_l l v DfracDiscarded).
+Proof. rewrite /PodTemplateSpecV.deepown_l. apply _. Qed.
+
+End persist.
